Finalize KeyAccValueList

Provenance/KeyAccValueList.lean
@@ -1,94 +1,203 @@
 import Mathlib.Data.List.Sort
 import Mathlib.Order.Defs.LinearOrder
 
-def LEByKey {α β: Type} [LinearOrder α] (a b: Prod α β) : Prop :=
+variable {α: Type} [LinearOrder α]
+
+def LEByKey (a b: Prod α β) : Prop :=
   a.fst <= b.fst
 
-instance [LinearOrder α] : DecidableRel (λ (a b: α×β) ↦ LEByKey a b) :=
+instance : DecidableRel (λ (a b: α×β) ↦ LEByKey a b) :=
   λ a b ↦ if h : a.fst <= b.fst then isTrue (h) else isFalse (h)
 
-instance [LinearOrder α] : IsTotal (α × β) LEByKey where
+instance : IsTotal (α × β) LEByKey where
   total := by
     intro a b
     unfold LEByKey
     exact le_total _ _
 
-instance [LinearOrder α] : IsTrans (α × β) LEByKey where
+instance : IsTrans (α × β) LEByKey where
   trans := by
     intro a b c
     unfold LEByKey
     exact Preorder.le_trans _ _ _
 
-class KeyAccValueList (α β: Type) [LinearOrder α] [DecidableEq β] [Add β] where
-  list : List (α × β)
-  sorted : list.Sorted LEByKey
-  noDupKey : list.Pairwise (·.fst≠·.fst)
+def KeyValueList (l : List (α×β)) := match l with
+| []     => True
+| hd::tl => KeyValueList tl ∧ match tl with
+  | []     => True
+  | hd'::_ => hd.1<hd'.1
 
-def KeyAccValueList.find? [LinearOrder α] [DecidableEq β] [Add β]
-  (l: KeyAccValueList α β) (a : α) : Option (α×β) :=
-  l.list.find? (·.fst=a)
+def List.addKV [DecidableEq β] [Add β] (l: List (α×β)) (a: α) (b: β) :=
+  match l.find? (·.1=a) with
+  | none        => l.orderedInsert LEByKey (a,b)
+  | some (a,b') => (l.eraseP (Prod.fst · = a)).orderedInsert LEByKey (a,b+b')
 
-def KeyAccValueList.erase [LinearOrder α] [DecidableEq β] [Add β]
-  (l: KeyAccValueList α β) (ab : α×β) : KeyAccValueList α β :=
-  {
-    list := l.list.erase ab
+theorem KeyValueList.sorted (l: List (α×β)) (h: KeyValueList l) :
+  List.Sorted LEByKey l := by
+    induction l with
+    | nil           => simp
+    | cons hd tl ih =>
+      apply List.sorted_cons.mpr
+      simp[KeyValueList] at h
+      constructor
+      . cases tl with
+        | nil          => simp
+        | cons hd' tl' =>
+          simp at h
+          intro b hb
+          rcases hb
+          . exact le_of_lt h.right
+          . rename_i hb
+            have sorted_tail := ih h.left
+            rw[List.sorted_cons] at sorted_tail
+            exact le_of_lt (lt_of_lt_of_le h.right (sorted_tail.left b hb))
+      . exact ih h.left
 
-    sorted := by
-      suffices
-        h : list.Sorted LEByKey → (list.erase ab).Sorted LEByKey
-        from h l.sorted
-      induction l.list with
-      | nil => simp
-      | cons hd tl ih =>
-        simp only [List.erase]
-        by_cases h₁ : hd == ab <;> simp only[h₁] <;> intro h
-        · exact List.Sorted.tail h
-        · simp at h₁
-          rw[List.sorted_cons]
-          constructor
-          . intro b hb
-            have : b ∈ tl := List.mem_of_mem_erase hb
-            exact (List.sorted_cons.mp h).left b this
-          . exact ih (List.Sorted.tail h)
+theorem KeyValueList.erase (l : List (α×β)) (h: KeyValueList l) (a: α):
+  KeyValueList (l.eraseP (·.1=a)) := by
+  induction l with
+  | nil           =>
+    unfold KeyValueList
+    simp
+  | cons hd tl ih =>
+    rw[List.eraseP_cons]
+    by_cases h' : hd.1=a
+    . simp[h']
+      exact h.left
+    . simp[h']
+      constructor
+      . exact ih h.left
+      . cases tl with
+        | nil          => simp
+        | cons hd' tl' =>
+          rw[List.eraseP_cons]
+          unfold KeyValueList at h
+          simp at h
+          by_cases h'': hd'.1=a
+          . simp[h'']
+            unfold KeyValueList at h
+            cases tl' with
+            | nil        => simp
+            | cons hd' _ =>
+              simp
+              simp at h
+              exact lt_trans h.right h.left.right
+          . simp[h'']
+            exact h.right
 
-    noDupKey := by
-      suffices
-        h : list.Pairwise (·.fst≠·.fst) → (list.erase ab).Pairwise (·.fst≠·.fst)
-        from h l.noDupKey
-      induction l.list with
-      | nil => simp
-      | cons hd tl ih =>
-        simp only [List.erase]
-        by_cases h₁ : hd == ab <;> simp only[h₁] <;> intro h
-        . exact (List.pairwise_cons.mp h).right
-        . simp at h₁
-          apply List.pairwise_cons.mpr
-          rw[List.pairwise_cons] at h
-          constructor
-          . intro a ha
-            have : a ∈ tl := List.mem_of_mem_erase ha
-            exact h.left a this
-          . exact ih h.right
-  }
+theorem KeyValueList.noKeyDup (l : List (α×β)) (h: KeyValueList l):
+  List.Pairwise (·.1≠·.1) l := by
+    induction l with
+    | nil => tauto
+    | cons hd tl ih =>
+      rw[List.pairwise_cons]
+      constructor
+      . unfold KeyValueList at h
+        induction tl with
+        | nil => tauto
+        | cons hd' tl' ih' =>
+          intro a' ha'
+          rcases ha'
+          . simp at h
+            exact ne_of_lt h.right
+          . rename_i ha'
+            have hb : KeyValueList tl' → List.Pairwise (·.1≠·.1) tl' := by
+              intro hb'
+              have := ih h.left
+              exact List.Pairwise.of_cons this
+            have hc: (KeyValueList tl' ∧ match tl' with | [] => True | hd' :: tail => hd.1 < hd'.1) := by
+              constructor
+              . exact h.left.left
+              . cases tl' with
+                | nil         => tauto
+                | cons hd'' _ =>
+                  simp
+                  simp at h
+                  have h'' := h.left.right
+                  simp at h''
+                  exact lt_trans h.right h''
+            exact ih' hb hc a' ha'
+      . exact ih h.left
 
-def KeyAccValueList.add [LinearOrder α] [DecidableEq β] [Add β]
-  (l: KeyAccValueList α β) (ab : α×β) : KeyAccValueList α β :=
-  {
-    list := match l.find? ab.fst with
-            | none       => l.list.orderedInsert LEByKey ab
-            | some (a,b) => (l.erase (a,b)).list.orderedInsert LEByKey ⟨ab.fst,ab.snd+b⟩
+theorem KeyValueList.erase_find (l : List (α×β)) (h: KeyValueList l) (a: α):
+  (l.eraseP (·.1=a)).find? (·.1=a) = none := by
+    induction l with
+    | nil => tauto
+    | cons hd tl ih =>
+      by_cases h' : hd.1 = a
+      . simp[h']
+        have hnoKeyDup := noKeyDup (hd::tl) h
+        rw[← h']
+        intro a' b ha'b
+        rw[List.pairwise_cons] at hnoKeyDup
+        have := hnoKeyDup.left (a',b) ha'b
+        simp[ne_comm] at this
+        assumption
+      . simp[h']
+        intro a' b ha'b
+        have hi := ih h.left
+        simp at hi
+        exact hi a' b ha'b
 
-    sorted :=
-      match l.find? ab.1 with
-      | none       => List.Sorted.orderedInsert _ _ l.sorted
-      | some (a,b) => List.Sorted.orderedInsert _ _ (l.erase (a,b)).sorted
+theorem KeyValueList.orderedInsert [DecidableEq β] [Add β]
+  (l : List (α×β)) (h: KeyValueList l) (a: α) (b: β) (hp: l.find? (·.1=a) = none):
+  KeyValueList (l.orderedInsert LEByKey (a,b)) := by
+    induction l with
+    | nil           => simp[KeyValueList]
+    | cons hd tl ih =>
+      simp[hp]
+      by_cases hab : a < hd.1 <;> simp[le_of_lt,hab,LEByKey]
+      . constructor
+        . exact h
+        . exact hab
+      . have hnle : ¬ a≤hd.1 := by
+          simp
+          simp at hab
+          simp at hp
+          exact lt_of_le_of_ne hab hp.left
+        simp[hnle]
+        unfold KeyValueList
+        constructor
+        . unfold List.addKV at ih
+          rw[List.find?_cons] at hp
+          have hne := ne_comm.mp (ne_of_not_le hnle)
+          simp[hne] at hp
+          have hfindtl : List.find? (·.1=a) tl = none := by
+            rw[List.find?_eq_none]
+            intro ab hab
+            simp
+            exact hp ab.1 ab.2 hab
+          simp[hfindtl] at ih
+          exact ih h.left
+        . cases tl with
+          | nil          => exact lt_of_not_le hnle
+          | cons hd' _   =>
+            simp
+            by_cases h'': a<=hd'.1 <;> simp[h'',LEByKey]
+            . exact lt_of_not_le hnle
+            . exact h.right
 
-    noDupKey := by
-      match h: l.find? ab.1 with
-      | none       =>
-        simp
-        unfold find? at h
-        simp[List.find?_eq_none] at h
-        sorry
-      | some (a,b) => sorry
-  }
+theorem KeyValueList.addKV [DecidableEq β] [Add β] (l : List (α×β)) (h: KeyValueList l) (a: α) (b: β):
+  KeyValueList (l.addKV a b) := by
+    induction l with
+    | nil           =>
+      unfold List.addKV
+      simp[KeyValueList]
+    | cons hd tl ih =>
+      unfold List.addKV
+      match h' : (hd::tl).find? (·.1=a) with
+      | none =>
+        simp[h']
+        exact KeyValueList.orderedInsert (hd::tl) h a b h'
+      | some (a,b') =>
+        simp[h']
+        have herasekvl : KeyValueList ((hd::tl).eraseP (·.1=a)) := by
+          exact erase (hd :: tl) h a
+        have herasefind : ((hd::tl).eraseP (·.1 = a)).find? (·.1=a) = none := by
+          exact erase_find (hd :: tl) h a
+        exact KeyValueList.orderedInsert
+          ((hd::tl).eraseP (·.1 = a))
+          herasekvl
+          a
+          (b+b')
+          herasefind
